src/functional/TreeSort.dfy
@@ -1,8 +1,15 @@
 include "./BST.dfy"
 
+/** Properties:
+
+  Lemma_TreeSortListIsOrdered(list)
+    ==> ensures list_is_ordered(TreeSort(list))
+
+  Lemma_TreeSortSameElemsThanList
+    ==> ensures List_ToMultiset(TreeSort(list)) == List_ToMultiset(list)
+
+ */
 function method TreeSort(list:List<int>) : (sortedList:List<int>)
-  // Lemma_TreeSortListIsOrdered(list) ==> ensures list_is_ordered(TreeSort(list))
-  // Lemma_TreeSortSameElemsThanList ==> ensures List_ToMultiset(TreeSort(list)) == List_ToMultiset(list)
   decreases list
 {
   BST_InOrder(BST_Load(list))
