test/fibonacci/Fibonacci.dfy
@@ -1,85 +1,85 @@
 include "../../src/fibonacci/Fibonacci.dfy"
 
 method Main() {
-  FibonacciRecursiveTest();
-  FibonacciTailRecursiveCallTest();
-  FibonacciRecursivePairTest();
-  FibonacciIterativeTest();
+  Fibonacci_RecursiveTest();
+  Fibonacci_TailRecursiveTest();
+  Fibonacci_RecursivePairTest();
+  Fibonacci_IterativeTest();
 }
 
-method FibonacciRecursiveTest() {
-  assert FibonacciRecursive(0) == 0;
-  assert FibonacciRecursive(1) == 1;
-  assert FibonacciRecursive(2) == 1;
-  assert FibonacciRecursive(3) == 2;
-  assert FibonacciRecursive(4) == 3;
-  assert FibonacciRecursive(5) == 5;
-  assert FibonacciRecursive(6) == 8;
-  assert FibonacciRecursive(7) == 13;
-  assert FibonacciRecursive(8) == 21;
-  assert FibonacciRecursive(9) == 34;
-  assert FibonacciRecursive(10) == 55;
-  assert FibonacciRecursive(11) == 89;
-  assert FibonacciRecursive(12) == 144;
+method Fibonacci_RecursiveTest() {
+  assert Fibonacci_Recursive(0) == 0;
+  assert Fibonacci_Recursive(1) == 1;
+  assert Fibonacci_Recursive(2) == 1;
+  assert Fibonacci_Recursive(3) == 2;
+  assert Fibonacci_Recursive(4) == 3;
+  assert Fibonacci_Recursive(5) == 5;
+  assert Fibonacci_Recursive(6) == 8;
+  assert Fibonacci_Recursive(7) == 13;
+  assert Fibonacci_Recursive(8) == 21;
+  assert Fibonacci_Recursive(9) == 34;
+  assert Fibonacci_Recursive(10) == 55;
+  assert Fibonacci_Recursive(11) == 89;
+  assert Fibonacci_Recursive(12) == 144;
 }
 
-method FibonacciTailRecursiveCallTest() {
-  assert FibonacciTailRecursive(0, 0, 1) == 0;
-  assert FibonacciTailRecursive(1, 0, 1) == 1;
-  assert FibonacciTailRecursive(2, 0, 1) == 1;
-  assert FibonacciTailRecursive(3, 0, 1) == 2;
-  assert FibonacciTailRecursive(4, 0, 1) == 3;
-  assert FibonacciTailRecursive(5, 0, 1) == 5;
-  assert FibonacciTailRecursive(6, 0, 1) == 8;
-  assert FibonacciTailRecursive(7, 0, 1) == 13;
-  assert FibonacciTailRecursive(8, 0, 1) == 21;
-  assert FibonacciTailRecursive(9, 0, 1) == 34;
-  assert FibonacciTailRecursive(10, 0, 1) == 55;
-  assert FibonacciTailRecursive(11, 0, 1) == 89;
-  assert FibonacciTailRecursive(12, 0 ,1) == 144;
+method Fibonacci_TailRecursiveTest() {
+  assert Fibonacci_TailRecursive(0, 0, 1) == 0;
+  assert Fibonacci_TailRecursive(1, 0, 1) == 1;
+  assert Fibonacci_TailRecursive(2, 0, 1) == 1;
+  assert Fibonacci_TailRecursive(3, 0, 1) == 2;
+  assert Fibonacci_TailRecursive(4, 0, 1) == 3;
+  assert Fibonacci_TailRecursive(5, 0, 1) == 5;
+  assert Fibonacci_TailRecursive(6, 0, 1) == 8;
+  assert Fibonacci_TailRecursive(7, 0, 1) == 13;
+  assert Fibonacci_TailRecursive(8, 0, 1) == 21;
+  assert Fibonacci_TailRecursive(9, 0, 1) == 34;
+  assert Fibonacci_TailRecursive(10, 0, 1) == 55;
+  assert Fibonacci_TailRecursive(11, 0, 1) == 89;
+  assert Fibonacci_TailRecursive(12, 0 ,1) == 144;
 }
 
-method FibonacciRecursivePairTest() {
-  assert FibonacciRecursivePair(0) == 0;
-  assert FibonacciRecursivePair(1) == 1;
-  assert FibonacciRecursivePair(2) == 1;
-  assert FibonacciRecursivePair(3) == 2;
-  assert FibonacciRecursivePair(4) == 3;
-  assert FibonacciRecursivePair(5) == 5;
-  assert FibonacciRecursivePair(6) == 8;
-  assert FibonacciRecursivePair(7) == 13;
-  assert FibonacciRecursivePair(8) == 21;
-  assert FibonacciRecursivePair(9) == 34;
-  assert FibonacciRecursivePair(10) == 55;
-  assert FibonacciRecursivePair(11) == 89;
-  assert FibonacciRecursivePair(12) == 144;
+method Fibonacci_RecursivePairTest() {
+  assert Fibonacci_RecursivePair(0) == 0;
+  assert Fibonacci_RecursivePair(1) == 1;
+  assert Fibonacci_RecursivePair(2) == 1;
+  assert Fibonacci_RecursivePair(3) == 2;
+  assert Fibonacci_RecursivePair(4) == 3;
+  assert Fibonacci_RecursivePair(5) == 5;
+  assert Fibonacci_RecursivePair(6) == 8;
+  assert Fibonacci_RecursivePair(7) == 13;
+  assert Fibonacci_RecursivePair(8) == 21;
+  assert Fibonacci_RecursivePair(9) == 34;
+  assert Fibonacci_RecursivePair(10) == 55;
+  assert Fibonacci_RecursivePair(11) == 89;
+  assert Fibonacci_RecursivePair(12) == 144;
 }
 
-method FibonacciIterativeTest() {
-  var fib := FibonacciIterative(0);
+method Fibonacci_IterativeTest() {
+  var fib := Fibonacci_Iterative(0);
   assert fib == 0;
-  fib := FibonacciIterative(1);
+  fib := Fibonacci_Iterative(1);
   assert fib == 1;
-  fib := FibonacciIterative(2);
+  fib := Fibonacci_Iterative(2);
   assert fib == 1;
-  fib := FibonacciIterative(3);
+  fib := Fibonacci_Iterative(3);
   assert fib == 2;
-  fib := FibonacciIterative(4);
+  fib := Fibonacci_Iterative(4);
   assert fib == 3;
-  fib := FibonacciIterative(5);
+  fib := Fibonacci_Iterative(5);
   assert fib == 5;
-  fib := FibonacciIterative(6);
+  fib := Fibonacci_Iterative(6);
   assert fib == 8;
-  fib := FibonacciIterative(7);
+  fib := Fibonacci_Iterative(7);
   assert fib == 13;
-  fib := FibonacciIterative(8);
+  fib := Fibonacci_Iterative(8);
   assert fib == 21;
-  fib := FibonacciIterative(9);
+  fib := Fibonacci_Iterative(9);
   assert fib == 34;
-  fib := FibonacciIterative(10);
+  fib := Fibonacci_Iterative(10);
   assert fib == 55;
-  fib := FibonacciIterative(11);
+  fib := Fibonacci_Iterative(11);
   assert fib == 89;
-  fib := FibonacciIterative(12);
+  fib := Fibonacci_Iterative(12);
   assert fib == 144;
 }
