test/imperative/InsertionSortTest.dfy
@@ -1,10 +1,10 @@
 include "../../src/imperative/InsertionSort.dfy"
 
 method Main() {
-  InsertionSortTest();
+  Test_InsertionSort();
 }
 
-method InsertionSortTest() {
+method Test_InsertionSort() {
   var A := new int[10];
   A[0], A[1], A[2], A[3], A[4], A[5], A[6], A[7], A[8], A[9] := 2, 4, 6, 15, 3, 19, 17, 16, 18, 1;
   InsertionSort(A);
