test/imperative/LinealSearchTest.dfy
@@ -1,10 +1,10 @@
 include "../../src/imperative/LinealSearch.dfy"
 
 method Main() {
-  LinealSearchTest();
+  Test_LinealSearch();
 }
 
-method LinealSearchTest() {
+method Test_LinealSearch() {
   var a := new int[10];
   a[0], a[1], a[2], a[3], a[4], a[5], a[6], a[7], a[8], a[9] := 2, 4, 6, 8, 10, 12, 14, 16, 18, 20;
   var index := LinealSearch(a, 12);
