test/imperative/TreeSortTest.dfy
@@ -1,10 +1,10 @@
 include "../../src/imperative/TreeSort.dfy"
 
 method Main() {
-  TreeSortTest();
+  Test_TreeSort();
 }
 
-method TreeSortTest() {
+method Test_TreeSort() {
   var list := Cons(2, Cons(10, Cons(4, Cons(12, Cons(7, List_Empty)))));
   var sorted := TreeSort(list);
   List_Print(sorted);
